theories/typechecker/examples_typechecker.v
@@ -1,0 +1,54 @@
+Require Import RecordUpdate.RecordUpdate.
+From stdpp Require Import base list.
+From Stdlib.Strings Require Import String.
+
+From RichWasm Require Import layout syntax typing util.
+From RichWasm Require Import typechecker.
+Set Bullet Behavior "Strict Subproofs".
+
+Definition ll_1_plus_2 := {|
+  m_imports := [];
+  m_functions := [{|
+    mf_type := (MonoFunT [] [(NumT (VALTYPE (AtomR I32R) ImCopy ImDrop) (IntT I32T))]);
+    mf_locals := [];
+    mf_body := [
+      (INumConst (InstrT [] [(NumT (VALTYPE (AtomR I32R) ImCopy ImDrop) (IntT I32T))]) 1);
+      (INumConst (InstrT [] [(NumT (VALTYPE (AtomR I32R) ImCopy ImDrop) (IntT I32T))]) 2);
+      (INum
+        (InstrT
+          [ (NumT (VALTYPE (AtomR I32R) ImCopy ImDrop) (IntT I32T));
+            (NumT (VALTYPE (AtomR I32R) ImCopy ImDrop) (IntT I32T))]
+          [ (NumT (VALTYPE (AtomR I32R) ImCopy ImDrop) (IntT I32T))])
+        (IInt2 I32T AddI))
+    ];
+  |}];
+  m_table := [];
+  m_exports := [{| me_name := "test"%string; me_desc := 0 |}];
+|}.
+
+Compute (has_module_type_checker_with_synth ll_1_plus_2).
+(* ==> inl () : type_checker_res *)
+
+Definition ll_1_plus_2_bad := {|
+  m_imports := [];
+  m_functions := [{|
+    mf_type := (MonoFunT [] [(NumT (VALTYPE (AtomR I32R) ImCopy ImDrop) (IntT I32T))]);
+    mf_locals := [];
+    mf_body := [
+      (INumConst (InstrT [] [(NumT (VALTYPE (AtomR I32R) ImCopy ImDrop) (IntT I32T))]) 1);
+      (INumConst (InstrT [] [(NumT (VALTYPE (AtomR I32R) ImCopy ImDrop) (IntT I64T))]) 2);
+      (INum
+        (InstrT
+          [ (NumT (VALTYPE (AtomR I32R) ImCopy ImDrop) (IntT I32T));
+            (NumT (VALTYPE (AtomR I32R) ImCopy ImDrop) (IntT I32T))]
+          [ (NumT (VALTYPE (AtomR I32R) ImCopy ImDrop) (IntT I32T))])
+        (IInt2 I32T AddI))
+    ];
+  |}];
+  m_table := [];
+  m_exports := [{| me_name := "test"%string; me_desc := 0 |}];
+|}.
+
+Compute (has_module_type_checker_with_synth ll_1_plus_2_bad).
+(* ==> inr "function types don't equal" : type_checker_res *)
+(* which I recognize isn't insanely helpful *)
